hfs

Arithmetization/ISigmaOne/HFS/PRF.lean
@@ -1,4 +1,4 @@
-import Arithmetization.ISigmaOne.HFS
+import Arithmetization.ISigmaOne.HFS.Seq
 
 /-!
 
@@ -201,110 +201,6 @@ instance result_definable_delta₁ : DefinableFunction ℒₒᵣ 𝚫₁ (fun v 
 end Construction
 
 end PR
-
-section seqExp
-
-lemma seqCons_le {x y s t : M} (hxy : x ≤ y) (hst : s ≤ t) :
-    s ⁀' x ≤ t + exp ((2 * t + y + 1)^2) := by
-  have : s ⁀' x ≤ t + exp ⟪2 * t, y⟫ := by
-    simp [seqCons]; exact insert_le_of_le_of_le (pair_le_pair (le_trans (lh_bound s) (by simp [hst])) hxy) hst
-  exact le_trans this (by simp)
-
-lemma seqProduct_exists_unique (s a : M) : ∃! t : M, ∀ x, x ∈ t ↔ ∃ v ∈ s, ∃ u ∈ a, x = v ⁀' u := by
-  have : 𝚺₁-Predicate fun x ↦ ∃ v ∈ s, ∃ u ∈ a, x = v ⁀' u := by definability
-  exact finite_comprehension₁! this ⟨log s + exp ((2 * log s + log a + 1)^2) + 1, by
-    rintro x ⟨v, hv, u, hu, rfl⟩
-    exact lt_succ_iff_le.mpr <| seqCons_le (le_log_of_mem hu) (le_log_of_mem hv)⟩
-
-def seqProduct (a s : M) : M := Classical.choose! (seqProduct_exists_unique a s)
-
-infixl:60 " ×ˢ " => seqProduct
-
-lemma mem_seqProduct_iff {x s a : M} : x ∈ s ×ˢ a ↔ ∃ v ∈ s, ∃ u ∈ a, x = v ⁀' u :=
-  Classical.choose!_spec (seqProduct_exists_unique s a) x
-
-lemma mem_seqProduct_iff' {u v a s : M} (Hv : Seq v) (Hs : ∀ w ∈ s, Seq w) :
-    v ⁀' u ∈ s ×ˢ a ↔ v ∈ s ∧ u ∈ a :=
-  ⟨by intro h
-      rcases mem_seqProduct_iff.mp h with ⟨v', hv', u', hu', e⟩
-      have : u = u' ∧ v = v' := by simpa [Hv, Hs v' hv'] using e
-      rcases this with ⟨rfl, rfl⟩
-      constructor <;> assumption,
-   by rintro ⟨hv, hu⟩
-      exact mem_seqProduct_iff.mpr ⟨v, hv, u, hu, rfl⟩⟩
-
-lemma mem_seqProduct_bound {x s a : M} (h : x ∈ s ×ˢ a) : x ≤ s + exp ((2 * s + a + 1)^2) := by
-  rcases mem_seqProduct_iff.mp h with ⟨v, hv, u, hu, rfl⟩
-  exact seqCons_le (le_of_lt <| lt_of_mem hu) (le_of_lt <| lt_of_mem hv)
-
-private lemma seqProduct_graph (t s a : M) :
-    t = s ×ˢ a ↔ ∃ e, e = exp ((2 * s + a + 1)^2) ∧ ∀ x ≤ t + s + e, x ∈ t ↔ ∃ v ∈ s, ∃ u ∈ a, x = v ⁀' u :=
-⟨by rintro rfl; exact ⟨exp ((2 * s + a + 1)^2), rfl, by intro x _; simp [mem_seqProduct_iff]⟩,
- by rintro ⟨_, rfl, h⟩
-    apply mem_ext; intro x
-    constructor
-    · intro hx;
-      exact mem_seqProduct_iff.mpr
-        <| h x (le_trans (le_of_lt <| lt_of_mem hx) (by simp [add_assoc])) |>.mp hx
-    · intro hx
-      exact h x (le_trans (mem_seqProduct_bound hx) <| by simp [add_assoc])
-        |>.mpr (mem_seqProduct_iff.mp hx)⟩
-
-def _root_.LO.FirstOrder.Arith.seqProductDef : 𝚺₁-Semisentence 3 := .mkSigma
-  “t s a | ∃ e, !expDef e (2 * s + a + 1)² ∧ ∀ x <⁺ t + s + e, x ∈ t ↔ ∃ v ∈' s, ∃ u ∈' a, !seqConsDef x v u”
-  (by simp [Hierarchy.iff_iff])
-
-lemma seqProduct_defined : 𝚺₁-Function₂ (seqProduct : M → M → M) via seqProductDef := by
-  intro v; simp [seqProductDef, seqProduct_graph]
-
-@[simp] lemma seqProduct_defined_iff (v) :
-    Semiformula.Evalbm M v seqProductDef.val ↔ v 0 = v 1 ×ˢ v 2 := seqProduct_defined.df.iff v
-
-instance seqProduct_definable : 𝚺₁-Function₂ (seqProduct : M → M → M) := Defined.to_definable _ seqProduct_defined
-
-def seqExp.formulae : PR.Formulae 1 where
-  zero := .mkSigma “y x | y = 1” (by simp)
-  succ := .mkSigma “y ih n x | !seqProductDef y ih x” (by simp)
-
-def seqExp.construction : PR.Construction M seqExp.formulae where
-  zero := fun _ ↦ {∅}
-  succ := fun a _ s ↦ s ×ˢ a 0
-  zero_defined := by intro v; simp [formulae, one_eq_singleton]
-  succ_defined := by intro v; simp [formulae]; rfl
-
-def seqExp (a k : M) : M := seqExp.construction.result ![a] k
-
-infix:80 " ^ˢ " => seqExp
-
-@[simp] lemma seqExp_zero (a : M) : a ^ˢ 0 = {∅} := by simp [seqExp, seqExp.construction]
-
-@[simp] lemma seqExp_succ (a k : M) : a ^ˢ (k + 1) = (a ^ˢ k) ×ˢ a := by simp [seqExp, seqExp.construction]
-
-def _root_.LO.FirstOrder.Arith.seqExpDef : 𝚺₁-Semisentence 3 := seqExp.formulae.resultDef |>.rew (Rew.substs ![#0, #2, #1])
-
-lemma seqExp_defined : 𝚺₁-Function₂ (seqExp : M → M → M) via seqExpDef :=
-  fun v ↦ by simp [seqExp.construction.result_defined_iff, seqExpDef]; rfl
-
-@[simp] lemma seqExp_defined_iff (v) :
-    Semiformula.Evalbm M v seqExpDef.val ↔ v 0 = v 1 ^ˢ v 2 := seqExp_defined.df.iff v
-
-instance seqExp_definable : 𝚺₁-Function₂ (seqExp : M → M → M) := Defined.to_definable _ seqExp_defined
-
-@[simp, definability] instance seqExp_definable' (Γ) : (Γ, m + 1)-Function₂ (seqExp : M → M → M) :=
-  .of_sigmaOne seqExp_definable _ _
-
-lemma seq_of_mem_seqExp {s a k : M} (h : s ∈ seqExp a k) : Seq s := by
-  induction k using induction_iSigmaOne generalizing s
-  · definability
-  case zero =>
-    have : s = ∅ := by simpa using h
-    simp [this]
-  case succ k ih =>
-    have : ∃ v ∈ a ^ˢ k, ∃ u ∈ a, s = v ⁀' u := by simpa [mem_seqProduct_iff] using h
-    rcases this with ⟨v, hv, u, _, rfl⟩
-    exact (ih hv).seqCons u
-
-end seqExp
 
 end LO.FirstOrder.Arith.Model
 
